<activity xml:id="act-ConnectingToAnotherSeries">
    <title>Connecting to Another Series</title>
    <introduction>
        <p>
            Let's start with some <q>known</q> series.
            <md>
                <mrow>\frac{1}{1-x} \amp = \sum_{k=0}^\infty x^k \amp \text{on }(-1,1)</mrow>
                <mrow>e^x \amp = \sum_{k=0}^\infty \frac{x^k}{k!} \amp \text{on } (-\infty,\infty)</mrow>
                <mrow>\sin(x) \amp = \sum_{k=0}^\infty \frac{(-1)^k x^{2k+1}}{(2k+1)!} \amp \text{on } (-\infty,\infty)</mrow>
                <mrow>\cos(x) \amp = \sum_{k=0}^\infty \frac{(-1)^k x^{2k}}{(2k)!} \amp \text{on } (-\infty,\infty)</mrow>
            </md>
            We're going to build a Taylor series for a logarithmic function:
            <me>
                y=\ln(1+x)
            </me>.
        </p>
    </introduction>
    <task>
        <statement>
            <p>
                In order to start, we're going to find a Taylor series for <m>g(x)=\dfrac{1}{1+x}</m>. Which of the <q>known</q> series above is this most similar to? How is it different?
            </p>
        </statement>
    </task>
    <task>
        <statement>
            <p>
                Find a Taylor series for <m>g(x)=\dfrac{1}{1+x}</m> by using <xref ref="thm-OperationsPowerSeries" text="type=global-title"/>. Can you connect this series to the known series by multiplying or composing something?
            </p>
        </statement>
        <hint>
            <p>
                Note that <m>1+x = 1-(-x)</m>.
            </p>
        </hint>
        <solution>
            <p>
                We're going to connect <m>g(x)=\dfrac{1}{1+x}</m> to the geometric Taylor series for <m>f(x) = \dfrac{1}{1-x}</m>. We can note that <m>g(x)=f(-x)</m>.
                <md>
                    <mrow>f(-x) \amp = \sum_{k=0}^\infty (-x)^k </mrow>
                    <mrow> \amp = \sum_{k=0}^{\infty} (-1)^k x^k</mrow>
                </md>
            </p>
        </solution>
    </task>
    <task>
        <statement>
            <p>
                Notice that the function we're trying to get a Taylor series for, <m>y=\ln(1+x)</m>, is an antiderivative of <m>g(x)=\dfrac{1}{1+x}</m>. Antidifferentiate the series you found above, using <xref ref="thm-DiffPowerSeries" text="type-global-title"/>. We know that at <m>x=0</m>, <m>y=0</m>, so use this information to find specific constant that we need when we antidifferentiate.
            </p>
        </statement>
        <solution>
            <p>
                <md>
                    <mrow>G(x) \amp = \int g(x)\;dx </mrow>
                    <mrow>G(x) \amp = \int \left(\sum_{k=0}^{\infty}(-1)^k x^k\right)\;dx</mrow>
                    <mrow> \amp = \sum_{k=0}^\infty (-1)^k \int x^k\;dx</mrow>
                    <mrow> \amp = \sum_{k=0}^\infty \frac{(-1)^k x^{k+1}}{k+1} + C</mrow>
                </md>
                We want <m>G(0)=0</m>, so we need to let <m>C=0</m>.
            </p>
            <p>
                So:
                <me>
                    \ln(1+x) = \sum_{k=0}^{\infty} \frac{(-1)^k x^{k+1}}{k+1}
                </me>.
                Sometimes this is written as:
                <me>
                    \ln(1+x) = \sum_{k=1}^{\infty} \frac{(-1)^{k+1} x^{k}}{k}
                </me>
            </p>
        </solution>
    </task>
    <task>
        <statement>
            <p>
                What is the interval of convergence for this new series? How does that relate to the interval of convergence of the <q>known</q> series you started with?
            </p>
        </statement>
        <solution>
            <p>
                We can apply the Ratio Test:

            <md>
                <mrow>\lim_{k\to\infty} \frac{|x|^{k+2}}{k+2}\cdot \frac{k+1}{|x|^{k+1}} \amp = \lim_{k\to\infty} \frac{|x|(k+1)}{k+2}</mrow>
                <mrow> \amp  = |x|</mrow>
            </md>
            So we know that the series will converge for <m>|x|\lt 1</m>. Now we can test the endpoints at <m>x=-1</m> and <m>x=1</m>.
            </p>
            <sidebyside widths="48% 48%">
                <p>
                    Case: <m>x=-1</m>
                    <me>
                        \sum_{k=0}^{\infty} \frac{-1}{k+1}
                    </me>
                    This is the negative harmonic series, and so the series diverges at <m>x=-1</m>.
                </p>
                <p>
                    Case: <m>x=1</m>
                    <me>
                        \sum_{k=0}^{\infty} \frac{(-1)^k}{k+1}
                    </me>
                    This is the alternating harmonic series, and so the series converges at <m>x=1</m>.
                </p>
            </sidebyside>
            <p>
                So, the interval of convergence is <m>(-1,1]</m>.
            </p>
        </solution>
    </task>    
</activity>