<?xml version="1.0" encoding="UTF-8"?>

<section xml:id="sec-BuildingTaylorSeries" xmlns:xi="http://www.w3.org/2001/XInclude">
  <title>How to Build Taylor Series</title>
  <introduction>
    <p>
      Let's first clear the air: we've been talking about <xref ref="def-PolynomialApproximation" text="custom">Taylor Polynomials</xref> that are partial sums of some larger infinite series. Then we talked about <xref ref="def-PowerSeries" text="title"/>, a generic structure of an infinite series of power functions of <m>x</m>. We want to combine these together, and name the specific power series that these Polynomial Approximations are partial sums of.
    </p>
    <definition xml:id="def-TaylorSeries">
      <title>Taylor Series</title>
      <statement>
        <p>
          If <m>f(x)</m> is an infinitely differentiable function at <m>x=a</m>, then the <term>Taylor series</term> expansion of <m>f(x)</m> centered at <m>x=a</m> is:
          <me>
            \sum_{k=0}^\infty \frac{f^{(k)}(a)}{k!}(x-a)^k
          </me>.
        </p>
      </statement>
    </definition>
    <aside>
      <p>
        If the Taylor series expansion of <m>f(x)</m> is centered at <m>x=0</m>, some people name these specifically, calling them <term>Maclaurin series</term>.  Colin Maclaurin made good use of Taylor series, and so is credited with having this special case named after him. 
      </p>
    </aside>
    <p>
      Now that we have named these Taylor series, we want to work on constructing these Taylor series for a given function. In this section, we'll investigate a couple of ways that we can do this.
    </p>
  </introduction>
  <subsection xml:id="subsec-Directly">
    <title>Constructing Directly</title>
    <p>
      We saw in <xref ref="sec-PolynomialApproximation" text="type-global-title"/> that we can use the idea of a polynomial partial sum to build out a Taylor series representation for a function.
    </p>
    <p>
      We'll need to build a bunch of terms for some Taylor polynomial, and then we can hopefully extrapolate afterwards. We want to come up with a general formula to define these terms, so that we can write the explicit formula in the infinite series, but we know that this, in general, is a difficult task! It's <em>hard</em> to find these explicit formulas for the terms in these series.
    </p>
    <p>
      It's not impossible, though! You can remind yourself of how we've done this! We found (and speculated about) the Taylor series for <m>f(x)=e^x</m>, <m>f(x)=\sin(x)</m>, and <m>f(x)=\cos(x)</m> (all centered at <m>x=0</m>) in <xref ref="act-BuildPolynomial" text="type-global-title"/> and <xref ref="act-PartialSumsOfWhat" text="type-global-title"/>.
    </p>
    <xi:include href="./activities/act-ConstructDirectly.ptx" />
  </subsection>
  <subsection xml:id="subsec-ConnectionsToOther">
    <title>Connections To Other Taylor Series</title>
    <p>
      A (hopefully) more useful strategy is to collect the Taylor series that we know, and then try to build a series for a function based on how that function relates. We saw this in <xref ref="thm-OperationsPowerSeries" text="type-global-title"/> and <xref ref="thm-DiffPowerSeries" text="type-global-title"/>.
    </p>
    <xi:include href="./activities/act-ConnectingToAnotherSeries.ptx" />
    <p>
      We're going to try this again with a different function as the goal!
    </p>
    <xi:include href="./activities/act-ConnectingToAnotherSeriesArcTan.ptx" />
    <p>
      Now we can update our list of <q>known</q> series!
    </p>
    <assemblage xml:id="strat-KnownSeries">
      <title>Known Taylor Series</title>
      <p>
        <md>
          <mrow>\frac{1}{1-x} \amp = \sum_{k=0}^\infty x^k \amp \text{on }(-1,1)</mrow>
          <mrow>e^x \amp = \sum_{k=0}^\infty \frac{x^k}{k!} \amp \text{on } (-\infty,\infty)</mrow>
          <mrow>\sin(x) \amp = \sum_{k=0}^\infty \frac{(-1)^k x^{2k+1}}{(2k+1)!} \amp \text{on } (-\infty,\infty)</mrow>
          <mrow>\cos(x) \amp = \sum_{k=0}^\infty \frac{(-1)^k x^{2k}}{(2k)!} \amp \text{on } (-\infty,\infty)</mrow>
          <mrow>\ln(1+x) \amp = \sum_{k=0}^\infty \frac{(-1)^k x^{k+1}}{k+1} \amp \text{on } (-1,1]</mrow>
          <mrow>\tan^{-1}(x) \amp = \sum_{k=0}^\infty \frac{(-1)^k x^{2k+1}}{2k+1} \amp \text{on } [-1,1]</mrow>
      </md>
      </p>
    </assemblage>
  </subsection>
</section>