<?xml version="1.0" encoding="UTF-8"?>

<section xml:id="sec-IntroSeries" xmlns:xi="http://www.w3.org/2001/XInclude">
  <title>Introduction to Infinite Series</title>

  <introduction>
    <p>
        Let's try to introduce the idea of an infinite series using a framework that we know and are (maybe) comfortable with: integrals!
    </p>
    <p>
        With an integral, we have a nice way of evaluating integrals of nicely behaved functions with finite limits of integration (<xref ref="thm-FTOC2" text="title"/>).
    </p>
    <p>
        Then, when we talked about improper integrals, we built a nice way to think about evaluating integrals with unbounded limits of integration (<xref ref="strat-ImproperIntegralsWidth" text="title"/>). How will we use this to think about infinite series, a sum of the infinitely many terms from an infinite sequence?
    </p>
  </introduction>
  <subsection xml:id="subsec-PartialSums">
    <title>Partial Sums</title>
      <p>
      If we approach infinite series in a manner similar to improper integrals, then we will need to do a couple of things.
      <ol>
        <li>
          <p>
            Truncate the infinite series at some finite ending point. This is what we did with the integral, when we replaced the infinity with some real number variable <m>t</m>. We might use <m>n</m> for the series "ending index."
          </p>
        </li>
        <li>
          <p>
            Find a formula for this truncated/finite version. For the integrals, we could use the <xref ref="thm-FTOC2" text="title"/> for this! For series, we'll need to do something else.
          </p>
        </li>
        <li>
          <p>
            Apply a limit as <m>t</m> (or <m>n</m> in the case of infinite series) goes off to infinity!
          </p>
        </li>
      </ol>
    </p>
    <xi:include href="./activities/act-IntroSeries.ptx" />
    <definition xml:id="def-PartialSum">
    <title>Partial Sum</title>
      <statement>
        <p>
          For an infinite series <m>\sum_{k=1}^\infty a_k</m>, we call <m>S_n = \sum_{k=1}^{n} a_k</m> the <m>n</m>th <term>Partial Sum</term> of the infinite series.
        </p>
      </statement>
    </definition>
    <definition xml:id="def-SeriesConvergence">
    <title>Series Convergence</title>
      <statement>
        <p>
          We say that the infinite series <m>\sum_{k=1}^\infty a_k</m> <term>converges</term> to the real number <m>L</m> if the sequence <m>\{S_n\}_{n=1}^\infty</m> converges to <m>L</m> (<m>\lim_{n\to\infty} S_n = L</m>), where <m>S_n = \sum_{k=1}^n a_k</m> is the <m>n</m>th partial sum of the infinite series.
        </p>
        <p>
          If the sequence of partial sums <m>\{S_n\}_{n=1}^\infty</m> diverges (the limit <m>\lim_{n\to\infty} S_n</m> does not exist), then we say that the infinite series <m>\sum_{k=1}^\infty a_k</m> <term>diverges</term>.
        </p>
      </statement>
    </definition>
  </subsection>
  <subsection xml:id="subsec-VisualizingPartialSums">
    <title>Visualizing the Sequence of Partial Sums</title>
    <p>
      Since we'll think about an infinite series <m>\sum_{k=0}^\infty a_k</m> as the sequence of its partial sums, <m>\left\{\sum_{k=0}^n a_k\right\}</m>, then we can think about visualizing an infinite series as really the same thing as visualizing a sequence in general (<xref ref="subsec-GraphingSequences"/>).
    </p>
    <p>
      Graphing examples.
    </p>
  </subsection>
  <subsection xml:id="subsec-SpecialSeries">
    <title>Special Series</title>
    <p>
      Let's look at three examples where we can think about partial sums and play with our new idea of series convergence.
    </p>
    <example>
    <introduction>
      <p>
        For each of the following series, write out a few of the terms of the series. Then write out the corresponding partial sums. Use these to find a formula for <m>S_n</m>, the <m>n</m>th partial sum. Then make a claim about whether or not the series converges and what it converges to.
      </p>
    </introduction>
    <task>
      <statement>
        <p>
          <m>\sum_{k=0}^\infty \left(\frac{1}{2^k}\right)</m>
        </p>
      </statement>
      <solution>
        <p>
          <md>
            <mrow> S_0 \amp = 1</mrow>
            <mrow> S_1 \amp = 1+\frac{1}{2} = \frac{3}{2}</mrow>
            <mrow> S_2 \amp = 1+\frac{1}{2}+\frac{1}{4} = \frac{7}{4} </mrow>
            <mrow>S_3 \amp = 1 + \frac{1}{2} + \frac{1}{4} + \frac{1}{8} = \frac{15}{8} </mrow>
            <mrow> S_n \amp = 1+ \frac{1}{2} + \frac{1}{4} + ... + \frac{1}{2^n} = \frac{2^{n+1}-1}{2^n} </mrow>
            <mrow> \amp = 2-\frac{1}{2^n}</mrow>
            <mrow>\lim_{n\to\infty} S_n \amp = \lim_{n\to\infty}\left(2 - \frac{1}{2^n}\right) </mrow>
            <mrow> \amp = 2</mrow>
          </md>
          The series converges to 2.
        </p>
      </solution>
    </task>
    <task>
      <statement>
        <p>
          <m>\sum_{k=2}^\infty \left(\frac{k}{\ln(k)} - \frac{k+1}{\ln(k+1)}\right)</m>
        </p>
      </statement>
      <solution>
        <p>
          <md>
            <mrow> S_2 \amp= \frac{2}{\ln(2)} - \frac{3}{\ln(3)} </mrow>
            <mrow> S_3 \amp = \frac{2}{\ln(2)} \underbrace{- \frac{3}{\ln(3)} + \frac{3}{\ln(3)}}_{0} - \frac{4}{\ln(4)}</mrow>
            <mrow> \amp = \frac{2}{\ln(2)} - \frac{4}{\ln(4)}</mrow>
            <mrow> S_4 \amp = \frac{2}{\ln(2)} \underbrace{- \frac{3}{\ln(3)} + \frac{3}{\ln(3)}}_{0} \underbrace{- \frac{4}{\ln(4)} + \frac{4}{\ln(4)}}_{0} - \frac{5}{\ln(5)}</mrow>
            <mrow> \amp = \frac{2}{\ln(2)} - \frac{5}{\ln(5)}</mrow>
            <mrow> S_5 \amp = \frac{2}{\ln(2)} \underbrace{- \frac{3}{\ln(3)} + \frac{3}{\ln(3)}}_{0} \underbrace{- \frac{4}{\ln(4)} + \frac{4}{\ln(4)}}_{0} \underbrace{- \frac{5}{\ln(5)} + \frac{6}{\ln(6)}}_{0} - \frac{6}{\ln(6)}</mrow>
            <mrow> \amp = \frac{2}{\ln(2)} - \frac{6}{\ln(6)}</mrow>
            <mrow> S_n \amp = \frac{2}{\ln(2)} \underbrace{- \frac{3}{\ln(3)} + \frac{3}{\ln(3)}}_{0} \underbrace{- \frac{4}{\ln(4)} + \frac{4}{\ln(4)}}_{0} \underbrace{- \frac{5}{\ln(5)} + ... + \frac{n}{\ln(n)}}_{0} - \frac{n+1}{\ln(n+1)}</mrow>
            <mrow> \amp = \frac{2}{\ln(2)} - \frac{n+1}{\ln(n+1)}</mrow>
            <mrow>\lim_{n\to\infty} S_n \amp =\lim_{n\to\infty} \frac{2}{\ln(2)} - \frac{n+1}{\ln(n+1)}</mrow>
            <mrow> \amp = -\infty</mrow>
          </md>
          So the series <m>\sum_{k=2}^\infty \left(\frac{k}{\ln(k)} - \frac{k+1}{\ln(k+1)}\right)</m> diverges.
        </p>
      </solution>
    </task>
    <task>
      <statement>
        <p>
          <m>\sum_{k=2}^\infty \left(\frac{2}{k^2-1}\right)</m> 
        </p>
      </statement>
      <hint>
        <p>
          This one is tricky! It's hard to notice anything unless we write out the series term formula a bit differently. Use <xref ref="sec-PartialFractions" text="title"/> to re-write <m>\frac{2}{k^2-1}</m> as <m>\frac{1}{k-1} - \frac{1}{k+1}</m>.
        </p>
      </hint>
      <solution>
        <p>
          <me>
            \sum_{k=2}^\infty \left(\frac{2}{k^2-1}\right) = \sum_{k=2}^\infty \left(\frac{1}{k-1} - \frac{1}{k+1}\right)
          </me>

          <md>
            <mrow> S_2 \amp = 1 - \frac{1}{3} </mrow>
            <mrow> S_3 \amp = 1 - \frac{1}{3} + \frac{1}{2} - \frac{1}{4} </mrow>
            <mrow> S_4 \amp = 1 - \frac{1}{3} + \frac{1}{2} - \frac{1}{4} + \frac{1}{3} - \frac{1}{5}</mrow>
            <mrow> \amp = 1 + \frac{1}{2} - \frac{1}{4} - \frac{1}{5}</mrow>
            <mrow> S_5 \amp = 1 - \frac{1}{3} + \frac{1}{2} - \frac{1}{4} + \frac{1}{3} - \frac{1}{5} + \frac{1}{4} - \frac{1}{6}</mrow>
            <mrow> \amp = 1 + \frac{1}{2} - \frac{1}{5} - \frac{1}{6}</mrow>
            <mrow>S_n \amp = 1 - \frac{1}{3} + \frac{1}{2} - \frac{1}{4} + \frac{1}{3} - \frac{1}{5} + \frac{1}{4} - \frac{1}{6} + ... + \underbrace{\frac{1}{n-2} - \frac{1}{n}}_{a_{n-1}} + \underbrace{\frac{1}{n-1} - \frac{1}{n+1}}_{a_{n}}</mrow>
            <mrow> \amp 1 + \frac{1}{2} - \frac{1}{n} - \frac{1}{n+2}</mrow>
            <mrow>\lim_{n\to\infty} S_n \amp = \lim_{n\to\infty} \left(1 + \frac{1}{2} - \frac{1}{n} - \frac{1}{n+2}\right) </mrow>
            <mrow> \amp = \frac{3}{2}</mrow>
          </md>
        </p>
      </solution>
    </task>
    </example>
    <p>
      These examples are a bit misleading: we often won't be able to do this kind of thing! For most infinite series, we will struggle to find an explicit formula for the <m>n</m>th partial sum. In these examples, though, we took advantage of some specific structure.
    </p>
    <p>
      In this first example (as well as the example in <xref ref="act-IntroSeries"/>), we noticed that because of the exponential function defining the terms, we were able to find some nice patterns in the partial sums. We'll explore this a bit more later in <xref ref="sec-CommonSeries"/>.
    </p>
    <p>
      Then in these other two examples, we noticed that once we could write each term as really a difference of two fractions that have a really similar structure, we got these "repeat" values from term to term where the opposite signs made things add up to 0. These are called "telescoping series," and they're mostly fun examples to think about partial sum formulas. We'll see some pop up later though, and Partial Fraction Decomposition is a nice trick to keep in mind for these kinds of things.
    </p>
  </subsection>
  

</section>