<exercises xml:id="ex-LimitsInvolvingInfinity">
    <exercise>
        <introduction>
            <p>
                Use the graph of the function <m>f(x)</m> below to determine each limit.
            </p>
            <figure xml:id="fig-ex-Infinity1">
                <caption>The function <m>f(x)</m>.</caption>
                <image source="./Limits/ex-Infinity1.png" width="70%">
                    <shortdescription>A rational function with a horizontal asymptote at y=0. At x=-3, the function increases up to a vertical asymptote and then decreases down from it. At x=5, the function increases up to a vertical asymptote and then increases away from it. At x=10 the function decreases towards a vertical asymptote and then decreases away from it.</shortdescription>
                </image>
            </figure>
        </introduction>
        <task>
            <statement>
                <p>
                    <m>\displaystyle\lim_{x\to-3^-} f(x)</m>
                </p>
            </statement>
            <solution>
                <p>
                    <m>\displaystyle\lim_{x\to-3^-} f(x) = \infty</m>
                </p>
            </solution>
        </task>
        <task>
            <statement>
                <p>
                    <m>\displaystyle\lim_{x\to-3^+} f(x)</m>
                </p>
            </statement>
            <solution>
                <p>
                    <m>\displaystyle\lim_{x\to-3^+} f(x) = \infty</m>
                </p>
            </solution>
        </task>
        <task>
            <statement>
                <p>
                    <m>\displaystyle\lim_{x\to-3} f(x)</m>
                </p>
            </statement>
            <solution>
                <p>
                    <m>\displaystyle\lim_{x\to-3} f(x) = \infty</m>
                </p>
            </solution>
        </task>
        <task>
            <statement>
                <p>
                    <m>\displaystyle\lim_{x\to5^-} f(x)</m>
                </p>
            </statement>
            <solution>
                <p>
                     <m>\displaystyle\lim_{x\to5^-} f(x) = \infty</m>
                </p>
            </solution>
        </task>
        <task>
            <statement>
                <p>
                    <m>\displaystyle\lim_{x\to5^+} f(x)</m>
                </p>
            </statement>
            <solution>
                <p>
                    <m>\displaystyle\lim_{x\to5^+} f(x) = -\infty</m>
                </p>
            </solution>
        </task>
        <task>
            <statement>
                <p>
                    <m>\displaystyle\lim_{x\to5} f(x)</m>
                </p>
            </statement>
            <solution>
                <p>
                    <m>\displaystyle\lim_{x\to5} f(x)</m> doesn't exist
                </p>
            </solution>
        </task>
        <task>
            <statement>
                <p>
                    <m>\displaystyle\lim_{x\to10^-} f(x)</m>
                </p>
            </statement>
            <solution>
                <p>
                    <m>\displaystyle\lim_{x\to10^-} f(x) = -\infty</m>
                </p>
            </solution>
        </task>
        <task>
            <statement>
                <p>
                    <m>\displaystyle\lim_{x\to10^+} f(x)</m>
                </p>
            </statement>
            <solution>
                <p>
                    <m>\displaystyle\lim_{x\to10^+} f(x) = \infty</m>
                </p>
            </solution>
        </task>
        <task>
            <statement>
                <p>
                    <m>\displaystyle\lim_{x\to10} f(x)</m>
                </p>
            </statement>
            <solution>
                <p>
                    <m>\displaystyle\lim_{x\to10} f(x)</m> doesn't exist
                </p>
            </solution>
        </task>
    </exercise>
    <exercise>
        <introduction>
            <p>
                Use the graph of the function <m>g(x)</m> below to determine each limit.
            </p>
            <figure xml:id="fig-ex-Infinity2">
                <caption>The function <m>g(x)</m>.</caption>
                <image source="./Limits/ex-Infinity2.png" width="70%">
                    <shortdescription>A graph of a function increasing away from a horizontal asymptote at x=-2 towards (0,0), and then decreasing towards a vertical asymptote at x=1. It decreases away from the vertical asymptote at x=1 towards a horizontal asymptote ay y=2.</shortdescription>
                </image>
            </figure>
        </introduction>
        <task>
            <statement>
                <p>
                    <m>\displaystyle\lim_{x\to-\infty}g(x)</m>
                </p>
            </statement>
            <solution>
                <p>
                    <m>\displaystyle\lim_{x\to-\infty}g(x) = -2</m>
                </p>
            </solution>
        </task>
        <task>
            <statement>
                <p>
                    <m>\displaystyle\lim_{x\to\infty}g(x)</m>
                </p>
            </statement>
            <solution>
                <p>
                    <m>\displaystyle\lim_{x\to\infty}g(x) =2</m>
                </p>
            </solution>
        </task>
    </exercise>
    <exercise>
        <introduction>
            <p>
                Use the graph of the function <m>h(x)</m> below to determine each limit.
            </p>
            <figure xml:id="fig-ex-Infinity3">
                <caption>The function <m>h(x)</m>.</caption>
                <image source="./Limits/ex-Infinity3.png" width="70%">
                    <shortdescription>A function increases from the bottom left corner of the graph towards an open point at (-1,0). Then it decreases away from a point at (-1,1) towards a horizontal asymptote at y=0.</shortdescription>
                </image>
            </figure>
        </introduction>
        <task>
            <statement>
                <p>
                    <m>\displaystyle\lim_{x\to-\infty}h(x)</m>
                </p>
            </statement>
            <solution>
                <p>
                    <m>\displaystyle\lim_{x\to-\infty}h(x) = -\inftry</m>
                </p>
            </solution>
        </task>
        <task>
            <statement>
                <p>
                    <m>\displaystyle\lim_{x\to\infty}h(x)</m>
                </p>
            </statement>
            <solution>
                <p>
                    <m>\displaystyle\lim_{x\to\infty}h(x) = 0</m>
                </p>
            </solution>
        </task>
    </exercise>
    <exercise>
        <introduction>
            <p>
                For each limit, fill in the table in a way that determines the limit, and report your answer.
            </p>
        </introduction>
        <task>
            <statement>
                <p>
                    <m>\displaystyle\lim_{x\to4^-} \left(\frac{3x}{x-4}\right)</m>
                </p>
                <tabular>
                    <row bottom="medium">
                        <cell halign="center"><m>x</m></cell>
                        <cell halign="center"><fillin characters="5" /></cell>
                        <cell halign="center"><fillin characters="5" /></cell>
                        <cell halign="center"><fillin characters="5" /></cell>
                        <cell halign="center"><m>4</m></cell>
                    </row>
                    <row>
                        <cell halign="center"><m>\frac{3x}{x-4}</m></cell>
                        <cell halign="center"><fillin characters="5" /></cell>
                        <cell halign="center"><fillin characters="5" /></cell>
                        <cell halign="center"><fillin characters="5" /></cell>
                        <cell halign="center">does not exist</cell>
                    </row>
                </tabular>
            </statement>
            <solution>
                <p>
                    <m>\displaystyle\lim_{x\to4^-} \left(\frac{3x}{x-4}\right) = -\infty</m>
                </p>
            </solution>
        </task>
        <task>
            <statement>
                <p>
                    <m>\displaystyle\lim_{x\to4^+} \left(\frac{3x}{x-4}\right)</m>
                </p>
                <tabular>
                    <row bottom="medium">
                        <cell halign="center"><m>x</m></cell>
                        <cell halign="center"><m>4</m></cell>
                        <cell halign="center"><fillin characters="5" /></cell>
                        <cell halign="center"><fillin characters="5" /></cell>
                        <cell halign="center"><fillin characters="5" /></cell>
                    </row>
                    <row>
                        <cell halign="center"><m>\frac{3x}{x-4}</m></cell>
                        <cell halign="center">does not exist</cell>
                        <cell halign="center"><fillin characters="5" /></cell>
                        <cell halign="center"><fillin characters="5" /></cell>
                        <cell halign="center"><fillin characters="5" /></cell>
                    </row>
                </tabular>
            </statement>
            <solution>
                <p>
                    <m>\displaystyle\lim_{x\to4^+} \left(\frac{3x}{x-4}\right) = \infty</m>
                </p>
            </solution>
        </task>
        <task>
            <statement>
                <p>
                    <m>\displaystyle\lim_{x\to 1} \left(\frac{x-3}{(2x-4)(x-1)^2}\right)</m>
                </p>
                <tabular>
                    <row bottom="medium">
                        <cell halign="center"><m>x</m></cell>
                        <cell halign="center"><fillin characters="5" /></cell>
                        <cell halign="center"><fillin characters="5" /></cell>
                        <cell halign="center"><fillin characters="5" /></cell>
                        <cell halign="center"><m>1</m></cell>
                        <cell halign="center"><fillin characters="5" /></cell>
                        <cell halign="center"><fillin characters="5" /></cell>
                        <cell halign="center"><fillin characters="5" /></cell>
                    </row>
                    <row>
                        <cell halign="center"><m>\frac{x-3}{(2x-4)(x-1)^2}</m></cell>   
                        <cell halign="center"><fillin characters="5" /></cell>
                        <cell halign="center"><fillin characters="5" /></cell>
                        <cell halign="center"><fillin characters="5" /></cell>
                        <cell halign="center">does not exist</cell>
                        <cell halign="center"><fillin characters="5" /></cell>
                        <cell halign="center"><fillin characters="5" /></cell>
                        <cell halign="center"><fillin characters="5" /></cell>                    
                    </row>
                </tabular>
            </statement>
            <solution>
                <p>
                     <m>\displaystyle\lim_{x\to 1} \left(\frac{x-3}{(2x-4)(x-1)^2}\right) = \infty</m>
                </p>
            </solution>
        </task>
    </exercise>
    <exercise>
        <introduction>
            <p>
                Evaluate the following limits analytically. Also evaluate the relevant one-sided limits when needed.
            </p>
        </introduction>
        <task>
            <statement>
                <p>
                   <m>\displaystyle\lim_{x\to-\infty} \left(2+4x-5x^2+\dfrac{x^3}{7} - \dfrac{8x^4}{9}\right)</m>
                </p>
            </statement>
            <solution>
                <p>
                    <m>\displaystyle\lim_{x\to-\infty} \left(2+4x-5x^2+\dfrac{x^3}{7} - \dfrac{8x^4}{9}\right) = -\infty</m>
                </p>
            </solution>
        </task>
        <task>
            <statement>
                <p>
                   <m>\displaystyle\lim_{x\to\infty} \left( \dfrac{5x^3-4x+3}{2x+6}\right)</m>
                </p>
            </statement>
            <solution>
                <p>
                    <m>\displaystyle\lim_{x\to\infty} \left( \dfrac{5x^3-4x+3}{2x+6}\right) = \infty</m>
                </p>
            </solution>
        </task>
        <task>
            <statement>
                <p>
                   <m>\displaystyle\lim_{x\to -3^-} \left( \dfrac{5x^3-4x+3}{2x+6}\right)</m>
                </p>
            </statement>
            <solution>
                <p>
                    <m>\displaystyle\lim_{x\to -3^-} \left( \dfrac{5x^3-4x+3}{2x+6}\right) = \infty</m>
                </p>
            </solution>
        </task>
        <task>
            <statement>
                <p>
                   <m>\displaystyle\lim_{x\to-\infty} \left( \dfrac{x-10}{3x+4}\right)</m>
                </p>
            </statement>
            <solution>
                <p>
                    <m>\displaystyle\lim_{x\to-\infty} \left( \dfrac{x-10}{3x+4}\right) = \frac{1}{3}</m>
                </p>
            </solution>
        </task>
        <task>
            <statement>
                <p>
                   <m>\displaystyle\lim_{x\to 2} \left( \dfrac{4x-1}{x^4-16}\right)</m>
                </p>
            </statement>
            <solution>
                <p>
                    <md>
                        <mrow>\lim_{x\to 2^-} \left( \dfrac{4x-1}{x^4-16}\right) \amp = -\infty </mrow>
                        <mrow>\lim_{x\to 2^+} \left( \dfrac{4x-1}{x^4-16}\right) \amp = \infty </mrow>
                    </md>
                </p>
            </solution>
        </task>
        <task>
            <statement>
                <p>
                   <m>\displaystyle\lim_{x\to\infty} \left( \dfrac{6-5x^5}{2+3x^2}\right)</m>
                </p>
            </statement>
            <solution>
                <p>
                    <m>\displaystyle\lim_{x\to\infty} \left( \dfrac{6-5x^5}{2+3x^2}\right) = -\infty</m>
                </p>
            </solution>
        </task>
        <task>
            <statement>
                <p>
                   <m>\displaystyle\lim_{x\to 1} \left( \dfrac{x^2+1}{x^3-2x^2+x}\right)</m>
                </p>
            </statement>
            <solution>
                <p>
                    <m>\displaystyle\lim_{x\to 1} \left( \dfrac{x^2+1}{x^3-2x^2+x}\right)=\infty</m>
                </p>
            </solution>
        </task>
        <task>
            <statement>
                <p>
                   <m>\displaystyle\lim_{\theta\to3\pi/2} \sin(\theta)\tan(\theta)</m>
                </p>
            </statement>
            <solution>
                <p>
                    <md>
                        <mrow>\lim_{\theta\to3\pi/2^-} \sin(\theta)\tan(\theta) \amp =-\infty</mrow>
                        <mrow>\lim_{\theta\to3\pi/2^+} \sin(\theta)\tan(\theta) \amp =\infty</mrow>
                    </md>
                </p>
            </solution>
        </task>
    </exercise>
    <exercise>
        <introduction>
            <p>
                For each of the following functions, find the locations of any vertical asymptotes and report the behavior of the functions around those asymptotes using limit statements.
            </p>
        </introduction>
        <task>
            <statement>
                <p>
                   <m>f(x) = \dfrac{|x-4|}{x+2}</m>
                </p>
            </statement>
        </task>
        <task>
            <statement>
                <p>
                   <m>g(x) = \dfrac{\sin x}{x^2-1}</m>
                </p>
            </statement>
        </task>
        <task>
            <statement>
                <p>
                   <m>h(t) = \dfrac{4}{t} + \dfrac{9}{t-1}</m>
                </p>
            </statement>
            <hint>
                <p>
                    If you'd rather, you can add the terms together to get:
                    <me>
                        h(t)=\frac{13t-4}{t(t-1)}
                    </me>.
                </p>
            </hint>
        </task>
        <task>
            <statement>
                <p>
                   <m>s(w) = \dfrac{w^3-3w^2+w-1}{w^2-5w+6}</m>
                </p>
            </statement>
        </task>
        <task>
            <statement>
                <p>
                   <m>f(x) = \dfrac{e^x}{(x-3)^4}</m>
                </p>
            </statement>
        </task>
    </exercise>
    <exercise>
        <introduction>
            <p>
                For each of the following functions, find the locations of any horizontal asymptotes using limit statements (as <m>x\to\infty</m> and <m>x\to-\infty</m>).
            </p>
        </introduction>
        <task>
            <statement>
                <p>
                   <m>f(x)= 2 + \dfrac{10}{x^2}</m>
                </p>
            </statement>
        </task>
        <task>
            <statement>
                <p>
                    <m>g(x)=\dfrac{4x^5-3x^3+5x-1}{10x^2+5x^3-5x^4}</m>
                </p>
            </statement>
        </task>
        <task>
            <statement>
                <p>
                    <m>h(x) = \dfrac{3x^2+4x+\sqrt{x}}{1-\sqrt{x}-2x^2}</m>
                </p>
            </statement>
        </task>
        <task>
            <statement>
                <p>
                    <m>j(x) = \dfrac{3}{5 + 10^{1/x}}</m>
                </p>
            </statement>
        </task>
    </exercise>
</exercises>